Complete example that doesn’t verify yet

text/Random.dfy
@@ -1,19 +1,42 @@
 module Random {
   trait RandomNumberGenerator {
+    ghost var Repr: set<object>
+    predicate Valid() 
+      reads this, Repr
+      ensures Valid() ==> this in Repr
+    {
+      this in Repr
+    }
     method Generate(max: nat) returns (res: nat) 
+      requires Valid()
       requires 0 < max
-      ensures 0 <= res < max
+      modifies Repr
+      ensures Valid()
+      ensures 0 <= res < max 
   }
 
+  // Goofy implementation that technically obeys the spec. :)
   class MyRandomNumberGenerator extends RandomNumberGenerator {
-    constructor() {}
+    var next: nat
+    constructor() 
+      ensures Valid() 
+      ensures fresh(Repr)
+    {
+      Repr := {this};
+    }
 
     method Generate(max: nat) returns (res: nat)
+      requires Valid()
       requires 0 < max
+      modifies Repr
+      ensures Valid()
       ensures 0 <= res < max 
     {
-      // What :)
-      return max / 2;
+      if next >= max {
+        next := 0;
+      }
+      res := next;
+      next := next + 1;
     }
   }
 }
