text/Test.dfy
@@ -1,27 +1,48 @@
 include "./Profiler.dfy"
 include "./Random.dfy"
+include "./Memoization.dfy"
 
 module Singletons {
 
   import opened Profiling
   import opened Random
+  import opened Memoization
 
   class Globals {
     var generator: RandomNumberGenerator?
     const profiler: Profiler
+    const fibonacciMemoized: Memoizer<nat, nat>
+    const factorialMemoized: Memoizer<nat, nat>
 
     constructor() 
       ensures profiler.Valid() 
       ensures fresh(profiler.Repr)
-      ensures generator != null
+      ensures generator != null && generator.Valid()
+      ensures fresh(generator.Repr)
+      ensures fibonacciMemoized.Valid()
+      ensures fresh(fibonacciMemoized)
+      ensures factorialMemoized.Valid()
+      ensures fresh(factorialMemoized)
     {
       profiler := new Profiler();
       generator := new MyRandomNumberGenerator();
-      
+      fibonacciMemoized := new Memoizer(n => Fibonacci(n));
+      factorialMemoized := new Memoizer(n => Factorial(n));
+
       new;
       
       profiler.AddLocation("Foo");
       profiler.AddLocation("Bar");
+    }
+
+    static function method Fibonacci(n: nat): nat
+    {
+      if n < 2 then n else Fibonacci(n-2) + Fibonacci(n-1)
+    }
+
+    static function method Factorial(n: nat): nat
+    {
+      if n == 0 then 1 else n * Factorial(n-1)
     }
   }
 
@@ -32,6 +53,8 @@ module Singletons {
 
     expect "Foo" in globals.profiler.locations;
     globals.profiler.RecordCall("Foo");
+
+    var tenthFactorial := globals.factorialMemoized.Apply(10);
   }
 }
 
